Makefile
@@ -5,8 +5,8 @@ ROCQC=rocq compile
 rocq:
 	$(ROCQC) Utils.v
 	$(ROCQC) LZ_Matching.v
-	$(ROCQC) LZ_Expand.v
 	$(ROCQC) LZ_Tokens.v
+	$(ROCQC) LZ_Expand.v
 	$(ROCQC) LZ.v
 
 clean:
